A type of label-free DAG with actions for nodes.
Test will be whether or not this type can be used to replay the
reasoning in the datadeps theory.

hol/dagScript.sml
@@ -9,224 +9,60 @@ val _ = new_theory "dag";
 
 val _ = type_abbrev("node", ``:(α,β,unit) action``)
 
-val geq_def = Define`
-  geq g1 g2 = ∃f. imap f g1 = g2
+val (geq_rules,geq_ind,geq_cases) = Hol_reln`
+  (∀g. geq g g) ∧
+  (∀g1 g2. geq g1 g2 ⇒ geq g2 g1) ∧
+  (∀g1 g2 g3. geq g1 g2 ∧ geq g2 g3 ⇒ geq g1 g3) ∧
+  (∀a g1 g2. geq g1 g2 ⇒ geq (a::g1) (a::g2)) ∧
+  (∀a:(α,β)node b:(α,β)node g. a ≁ₜ b ⇒ geq (a::b::g) (b::a::g))
 `;
 
 val geq_refl = store_thm(
   "geq_refl[simp]",
   ``geq g g``,
-  simp[geq_def] >> qexists_tac `λx.x` >> simp[]);
-
-val sym_lemma = prove(
-  ``INJ f (s:α set) univ(:β) ⇒
-    ∃f'. INJ f' (IMAGE f s) univ(:α) ∧ ∀x. x ∈ s ⇒ f' (f x) = x``,
-  strip_tac >>
-  `SURJ f s (IMAGE f s)` by simp[] >>
-  IMP_RES_THEN (qx_choose_then `g` strip_assume_tac) SURJ_INJ_INV >>
-  qexists_tac `g` >> fs[PULL_EXISTS] >>
-  conj_tac >- (match_mp_tac INJ_SUBSET >>
-               map_every qexists_tac [`IMAGE f s`, `s`] >> simp[]) >>
-  fs[INJ_THM] >> metis_tac[]);
-
-val sym_lemma2 = prove(
-  ``∀g f. ∃f'. imap f' (imap f g) = g``,
-  rpt gen_tac >> reverse (Cases_on `INJ f (idents g) UNIV`)
-  >- (simp[imap_id] >> qexists_tac `λx.x` >> simp[]) >>
-  IMP_RES_THEN (qx_choose_then `f2` strip_assume_tac) sym_lemma >>
-  qexists_tac `f2` >>
-  `INJ (f2 o f) (idents g) UNIV` by simp[INJ_DEF] >>
-  simp[imap_imap_o] >> simp[Cong imap_CONG])
+  simp[geq_rules]);
 
 val geq_sym = store_thm(
   "geq_sym",
   ``geq g1 g2 ⇔ geq g2 g1``,
-  rw[geq_def, EQ_IMP_THM] >> metis_tac[sym_lemma2]);
+  metis_tac[geq_rules])
 
 val geq_trans = store_thm(
   "geq_trans",
   ``geq g1 g2 ∧ geq g2 g3 ⇒ geq g1 g3``,
-  simp[geq_def] >>
-  disch_then (CONJUNCTS_THEN2 (qx_choose_then `f1` assume_tac)
-                              (qx_choose_then `f2` assume_tac)) >>
-  reverse (Cases_on `INJ f1 (idents g1) UNIV`)
-  >- (fs[imap_id] >> metis_tac[]) >>
-  reverse (Cases_on `INJ f2 (idents g2) UNIV`)
-  >- (fs[imap_id] >> metis_tac[]) >>
-  `INJ f1 (idents g1) (idents g2)` by (rw[idents_imap] >> fs[INJ_THM]) >>
-  `INJ (f2 o f1) (idents g1) UNIV` by metis_tac[INJ_COMPOSE] >>
-  qexists_tac `f2 o f1` >> simp[GSYM imap_imap_o]);
+  metis_tac[geq_rules]);
 
-val dagAdd0_def = Define`
-  dagAdd0 (a:(α,β,unit) action) g =
-    <| writes := a.writes ; reads := a.reads ;
-       data := a.data; ident := LEAST n. n ∉ idents g |> ⊕ g
+val dagmap0_def = Define`
+  dagmap0 f g = MAP (polydata_upd f) g
 `;
 
-val FINITE_idents = store_thm(
-  "FINITE_idents[simp]",
-  ``FINITE (idents g)``,
-  simp[idents_thm]);
+val dagmap0_thm = prove(
+  ``dagmap0 f [] = [] ∧
+    dagmap0 f (a::g) = polydata_upd f a :: dagmap0 f g``,
+  simp[dagmap0_def]);
 
-val idents_has_nonmembers = prove(
-  ``∀g:(α,β,num) G. ∃n. n ∉ idents g``,
-  metis_tac[INFINITE_NUM_UNIV, FINITE_idents, IN_INFINITE_NOT_FINITE]);
-
-val wfdagAdd = prove(
-  ``∀a g1 g2. geq g1 g2 ⇒ geq (dagAdd0 a g1) (dagAdd0 a g2)``,
-  rpt gen_tac >> simp[geq_def, dagAdd0_def] >>
-  disch_then (qx_choose_then `f` assume_tac) >>
-  reverse (Cases_on `INJ f (idents g1) UNIV`) >> fs[imap_id]
-  >- (qexists_tac `λx. x` >> simp[]) >>
-  qabbrev_tac `m = LEAST n. n ∉ idents g1` >>
-  qabbrev_tac `n = LEAST n. n ∉ idents g2` >>
-  qabbrev_tac `f2 = λi. if i = m then n else f i` >>
-  qexists_tac `f2` >>
-  `m ∉ idents g1 ∧ n ∉ idents g2`
-    by (conj_tac >> simp[Abbr`m`, Abbr`n`] >> numLib.LEAST_ELIM_TAC >>
-        simp[idents_has_nonmembers]) >>
-  `∀i. i ∈ idents g1 ⇒ i ≠ m` by metis_tac[] >>
-  `∀i. i ∈ idents g1 ⇒ f i ∈ idents g2` by rw[idents_imap] >>
-  `INJ f2 (m INSERT idents g1) UNIV`
-    by (dsimp[INJ_DEF, Abbr`f2`] >> fs[INJ_THM] >> metis_tac[]) >>
-  simp[imap_add_action] >>
-  `∀i. i ∈ idents g1 ⇒ f2 i = f i` by simp[Abbr`f2`] >>
-  `f2 m = n` by simp[Abbr`f2`] >>
-  simp[Cong imap_CONG] >> asm_simp_tac (bool_ss ++ ETA_ss) []);
-
-val imap_dgmap = store_thm(
-  "imap_dgmap",
-  ``∀G f g. imap f (dgmap g G) = dgmap g (imap f G)``,
-  ho_match_mp_tac graph_ind >> simp[] >> map_every qx_gen_tac [`a`, `G`] >>
-  strip_tac >> map_every qx_gen_tac [`f`, `g`] >>
-  reverse (Cases_on `INJ f (a.ident INSERT idents G) UNIV`)
-  >- simp[imap_id] >>
-  simp[imap_add_action] >> simp[polydata_upd_def])
-
-val wfdgmap = prove(
-  ``∀f g1 g2. geq g1 g2 ⇒ geq (dgmap f g1) (dgmap f g2)``,
-  rpt gen_tac >> simp[geq_def, imap_dgmap] >>
-  disch_then (qx_choose_then `f2` (SUBST_ALL_TAC o SYM)) >> metis_tac[]);
-
-val dgmap_dagAdd0 = prove(
-  ``dgmap f (dagAdd0 a g) = dagAdd0 (polydata_upd f a) (dgmap f g)``,
-  simp[dagAdd0_def, polydata_upd_def]);
+val wfdagmap0 = prove(
+  ``∀g1 g2. geq g1 g2 ⇒ geq (dagmap0 f g1) (dagmap0 f g2)``,
+  Induct_on `geq` >> simp[geq_rules, dagmap0_def] >> metis_tac[geq_rules]);
 
 val geq_equiv = prove(
   ``∀g1 g2. geq g1 g2 ⇔ (geq g1 = geq g2)``,
   simp[FUN_EQ_THM] >> metis_tac[geq_refl, geq_sym, geq_trans]);
 
-val ginst = INST_TYPE [gamma |-> ``:num``]
-
-val nullident_def = Define`
-  nullident a = <| writes := a.writes; reads := a.reads; data := a.data;
-                   ident := () |>
-`;
-
-val nullident_ident_upd = prove(
-  ``nullident (a with ident updated_by f) = nullident a``,
-  simp[nullident_def,oneTheory.one]);
-
-val nodebag0_def = Define`
-  nodebag0 G = gEVAL (BAG_INSERT o nullident) {||} G
-`;
-
-val wfnodebag = prove(
-  ``∀g1 g2. geq g1 g2 ⇒ nodebag0 g1 = nodebag0 g2``,
-  simp[geq_def, nodebag0_def] >> rw[] >>
-  simp[gEVAL_imap_irrelevance, nullident_ident_upd,
-       BAG_INSERT_commutes]);
-
-val nodebag_emptydag0 = prove(
-  ``nodebag0 (emptyG : (α,β,num) G) = {||}``,
-  simp[BAG_INSERT_commutes, gEVAL_thm, nodebag0_def]);
-
-val gE_BI = prove(
-  ``gEVAL (BAG_INSERT o nullident) acc emptyG = acc ∧
-    (a.ident ∉ idents g ⇒
-      gEVAL (BAG_INSERT o nullident) acc (a ⊕ g) =
-      gEVAL (BAG_INSERT o nullident) (BAG_INSERT (nullident a) acc) g)``,
-  simp[gEVAL_thm, BAG_INSERT_commutes]);
-
-val dagAdd_lemma = prove(
-  ``∀g acc. gEVAL (BAG_INSERT o nullident) acc g =
-            acc ⊎ gEVAL (BAG_INSERT o nullident) {||} g``,
-  ho_match_mp_tac graph_ind >> conj_tac >- simp[] >>
-  rpt strip_tac >>
-  first_x_assum ((fn th => (simp[gE_BI] >> assume_tac th)) o
-                 assert (is_forall o concl)) >>
-  pop_assum (fn th => ONCE_REWRITE_TAC [th]) >>
-  simp[BAG_UNION_INSERT]);
-
-val nodebag_dagAdd0 = prove(
-  ``nodebag0 (dagAdd0 a g) = BAG_INSERT a (nodebag0 g)``,
-  simp[nodebag0_def, dagAdd0_def] >>
-  `(LEAST n. n ∉ idents g) ∉ idents g`
-    by (numLib.LEAST_ELIM_TAC >> simp[idents_has_nonmembers]) >>
-  simp[gE_BI, Once dagAdd_lemma] >> simp[BAG_UNION_INSERT] >>
-  simp[nullident_def, action_component_equality, oneTheory.one]);
-
-val nodebag_FINITE00 = prove(
-  ``∀g a. FINITE_BAG a ⇒ FINITE_BAG (gEVAL (BAG_INSERT o nullident) a g)``,
-  ho_match_mp_tac graph_ind >> simp[gE_BI]);
-
-val nodebag_FINITE0 = prove(
-  ``FINITE_BAG (nodebag0 g)``,
-  simp[nodebag_FINITE00, nodebag0_def]);
-
-val dagAdd_commutes0 = prove(
-  ``a ≁ₜ b ⇒ geq (dagAdd0 a (dagAdd0 b g)) (dagAdd0 b (dagAdd0 a g))``,
-  simp[dagAdd0_def] >>
-  qabbrev_tac `m = LEAST n. n ∉ idents g` >>
-  qabbrev_tac `n = LEAST n. n ≠ m ∧ n ∉ idents g` >>
-  `m ∉ idents g ∧ (m ≠ n ∧ n ∉ idents g)`
-    by (conj_tac >| [simp[Abbr`m`], simp[Abbr`n`]] >>
-        numLib.LEAST_ELIM_TAC >> simp[] >>
-        metis_tac[INFINITE_NUM_UNIV, FINITE_idents, IN_INFINITE_NOT_FINITE,
-                  IN_INSERT, FINITE_INSERT]) >>
-  simp[geq_def] >> strip_tac >>
-  qabbrev_tac `A = λi:num. <| writes := a.writes; reads := a.reads; data := a.data;
-                              ident := i |>` >>
-  qabbrev_tac `B = λi:num. <| writes := b.writes; reads := b.reads; data := b.data;
-                              ident := i |>` >>
-  simp[] >>
-  qabbrev_tac `f = λi. if i = n then m else if i = m then n else i` >>
-  `f n = m ∧ f m = n ∧ ∀i. i ∈ idents g ⇒ f i = i`
-    by (simp[Abbr`f`] >> metis_tac[]) >>
-  `∀i h. (A i).ident = i ∧ (B i).ident = i ∧
-         A i with ident updated_by h = A (h i) ∧
-         B i with ident updated_by h = B (h i)` by simp[Abbr`B`, Abbr`A`] >>
-  `INJ f (n INSERT m INSERT idents g) UNIV` by simp[INJ_DEF, Abbr`f`] >>
-  `INJ f (m INSERT idents g) UNIV` by fs[INJ_INSERT] >>
-  qexists_tac `f` >> simp[imap_add_action] >> simp[Cong imap_CONG] >>
-  simp[graph_equality, add_action_edges] >> rpt strip_tac
-  >- metis_tac[] >>
-  `∀i j. A i ≁ₜ B j` by (simp[Abbr`A`, Abbr`B`] >> fs[touches_def]) >>
-  metis_tac[touches_SYM, IN_edges])
-
-val dag_ind0 = prove(
-  ``∀P::respects (geq ===> (=)).
-        P (emptyG : (α,β,num)G) ∧
-        (∀a d. P d ⇒ P (dagAdd0 a d)) ⇒
-        ∀d. P d``,
-  simp[RES_FORALL_THM, quotientTheory.respects_def,
-       quotientTheory.FUN_REL, combinTheory.W_DEF] >>
-  ntac 3 strip_tac >> ho_match_mp_tac graph_ind >> simp[] >>
-  map_every qx_gen_tac [`a`, `d`] >> strip_tac >>
-  `geq (a ⊕ d) (dagAdd0 (nullident a) d)` suffices_by metis_tac[] >>
-  simp[geq_def] >>
-  qabbrev_tac `n = LEAST n. n ∉ idents d` >>
-  `n ∉ idents d`
-    by (simp[Abbr`n`] >>
-        numLib.LEAST_ELIM_TAC >> simp[idents_has_nonmembers]) >>
-  qabbrev_tac `f = λi. if i = a.ident then n else i` >>
-  `INJ f (a.ident INSERT idents d) UNIV`
-    by (simp[INJ_DEF,Abbr`f`] >> metis_tac[]) >>
-  `∀i. i ∈ idents d ⇒ f i = i` by (simp[Abbr`f`] >> metis_tac[]) >>
-  qexists_tac `f` >>
-  simp[imap_add_action, Cong imap_CONG, dagAdd0_def, nullident_def] >>
-  Q.ISPEC_THEN `a` strip_assume_tac action_literal_nchotomy >>
-  simp[Abbr`f`])
+val recursion = prove(
+  ``(∀a b r. a ≁ₜ b ⇒ f a (f b r) = f b (f a r)) ⇒
+    ∃h :: respects (geq ===> (=)).
+      (h [] = (e:γ)) ∧
+      (∀a:(α,β)node d. h (a::d) = f a (h d))``,
+  simp[quotientTheory.respects_def, quotientTheory.FUN_REL,
+       combinTheory.W_DEF, RES_EXISTS_THM] >> strip_tac >>
+  qx_choose_then `h` strip_assume_tac
+    (TypeBase.axiom_of ``:'a list``
+       |> ISPEC ``e:γ``
+       |> ISPEC ``λa:(α,β)node l:(α,β)node list r:γ. f a r : γ``
+       |> BETA_RULE) >>
+  qexists_tac `h` >> simp[] >> Induct_on `geq` >> simp[] >>
+  metis_tac[]);
 
 fun define_quotient {types,defs,thms,poly_preserves,poly_respects,respects} =
     let
@@ -243,71 +79,197 @@ fun define_quotient {types,defs,thms,poly_preserves,poly_respects,respects} =
       map save_thm named_new
     end
 
-val [dagmap_emptydag, dagmap_dagAdd, nodebag_emptydag, nodebag_dagAdd,
-     nodebag_FINITE, dagAdd_commutes, dag_ind] =
+val dagAdd_commutes0 = last (CONJUNCTS geq_rules)
+val wfdagAdd = List.nth(CONJUNCTS geq_rules, 3)
+val alpha_node = inst [alpha |-> ``:(α,β)node``]
+
+val [dag_ind, dag_recursion, dagAdd_commutes] =
   define_quotient {
-  types = [{name = "dag", equiv = ginst geq_equiv}],
-  defs = [("emptydag",``emptyG : (α,β,num)G``),
+  types = [{name = "dag", equiv = geq_equiv}],
+  defs = [("emptydag",``[] : (α,β)node list``),
           ("dagAdd",
-           ``dagAdd0 : (α,β,unit) action -> (α,β,num)G -> (α,β,num) G``),
-          ("dagmap", ``dgmap : (α -> γ) -> (α,β,num) G -> (γ,β,num) G``),
-          ("nodebag", ``nodebag0 : (α,β,num) G -> (α,β)node bag``)],
-  thms = [("dagmap_emptydag",
-           SIMP_CONV bool_ss [dgmap_emptyG]
-                     ``dgmap (f : α -> γ) (emptyG : (α,β,num) G)``),
-          ("dagmap_dagAdd", dgmap_dagAdd0),
-          ("nodebag_emptydag", nodebag_emptydag0),
-          ("nodebag_dagAdd", nodebag_dagAdd0),
-          ("nodebag_FINITE", ginst nodebag_FINITE0),
-          ("dagAdd_commutes", dagAdd_commutes0),
-          ("dag_ind", dag_ind0)],
+           ``CONS : (α,β) node -> (α,β) node list -> (α,β)node list``),
+          ("dagmap",
+           ``dagmap0 : (α -> γ) -> (α,β) node list -> (γ,β)node list``)],
+  thms = [("dag_ind", TypeBase.induction_of ``:'a list``
+                        |> INST_TYPE [alpha |-> ``:(α,β)node``]),
+          ("dag_recursion", recursion),
+          ("dagAdd_commutes", dagAdd_commutes0)],
   poly_preserves = [],
   poly_respects = [],
-  respects = [wfdgmap, wfdagAdd, wfnodebag]}
+  respects = [wfdagmap0, wfdagAdd]}
 
-val _ = export_rewrites ["nodebag_emptydag", "nodebag_FINITE",
-                         "nodebag_dagAdd", "dagmap_emptydag",
-                         "dagmap_dagAdd"]
+val _ = overload_on("ε", ``emptydag``)
+val _ = set_mapped_fixity {term_name = "dagAdd", tok = "<+",
+                           fixity = Infixr 501}
 
 val dag_CASES = store_thm(
   "dag_CASES",
-  ``∀d. d = emptydag ∨ ∃a d0. d = dagAdd a d0``,
+  ``∀d. d = emptydag ∨ ∃a d0. d = a <+ d0``,
   ho_match_mp_tac dag_ind >> simp[] >> metis_tac[]);
+
+val nodebag_def = new_specification("nodebag_def",
+  ["nodebag"],
+  dag_recursion |> ISPEC (alpha_node ``BAG_INSERT``)
+                |> SPEC (alpha_node ``{||}``)
+                |> SIMP_RULE (srw_ss()) [BAG_INSERT_commutes]);
+val _ = export_rewrites ["nodebag_def"]
+
+val FINITE_nodebag = store_thm(
+  "FINITE_nodebag[simp]",
+  ``∀d. FINITE_BAG (nodebag d)``,
+  ho_match_mp_tac dag_ind >> simp[]);
+
+val nodeset_def = new_specification("nodeset_def",
+  ["nodeset"],
+  dag_recursion |> ISPEC (alpha_node ``(INSERT)``)
+                |> SPEC (alpha_node ``∅``)
+                |> SIMP_RULE (srw_ss()) [INSERT_COMM])
+val _ = export_rewrites ["nodeset_def"]
+val _ = overload_on("IN", ``λa d. a ∈ nodeset d``)
+
+val FINITE_nodeset = store_thm(
+  "FINITE_nodeset[simp]",
+  ``∀d. FINITE (nodeset d)``,
+  ho_match_mp_tac dag_ind >> simp[]);
+
+val dagsize_def = new_specification("dagsize_def",
+  ["dagsize"],
+  dag_recursion |> ISPEC ``λa:(α,β)node r. r + 1`` |> SPEC ``0n``
+                |> SIMP_RULE (srw_ss()) [])
+val _ = export_rewrites ["dagsize_def"]
 
 val dag_distinct = store_thm(
   "dag_distinct[simp]",
   ``emptydag ≠ dagAdd a d``,
-  disch_then (mp_tac o Q.AP_TERM `nodebag`) >> simp[]);
+  disch_then (mp_tac o Q.AP_TERM `dagsize`) >> simp[]);
 
-val dagsize_def = Define`dagsize d = BAG_CARD (nodebag d)`
+val dagsize_EQ0 = store_thm(
+  "dagsize_EQ0[simp]",
+  ``(dagsize d = 0 ⇔ d = emptydag) ∧ (0 = dagsize d ⇔ d = emptydag)``,
+  qspec_then `d` strip_assume_tac dag_CASES >> simp[]);
 
-val dagsize_thm = store_thm(
-  "dagsize_thm[simp]",
-  ``dagsize emptydag = 0 ∧
-    dagsize (dagAdd a d) = 1 + dagsize d``,
-  simp[dagsize_def, BAG_CARD_THM]);
+val nodebag_EQ_EMPTY = store_thm(
+  "nodebag_EQ_EMPTY[simp]",
+  ``(nodebag g = {||} ⇔ g = emptydag) ∧
+    ({||} = nodebag g ⇔ g = emptydag)``,
+  qspec_then `g` strip_assume_tac dag_CASES >> simp[]);
 
-val (dagEVALR_rules, dagEVALR_ind, dagEVALR_cases) = Hol_reln`
-  (∀acc. dagEVAL opn acc emptydag acc)
+val dagAdd_commutes' = prove(
+  ``b ≁ₜ a ⇒ a <+ b <+ g = b <+ a <+ g``,
+  metis_tac[touches_SYM, dagAdd_commutes]);
 
-     ∧
+val dagmap_def = new_specification("dagmap_def",
+  ["dagmap"],
+  dag_recursion |> ISPEC ``dagAdd o polydata_upd f`` |> SPEC ``emptydag``
+                |> SIMP_RULE (srw_ss()) [dagAdd_commutes']
+                |> Q.GEN `f` |> SIMP_RULE bool_ss [SKOLEM_THM]
+                |> SIMP_RULE bool_ss [FORALL_AND_THM]);
+val _ = export_rewrites ["dagmap_def"]
 
-  (∀a acc d r.
-      dagEVAL opn (opn a acc) d r ⇒
-      dagEVAL opn acc (dagAdd a d) r)
-`;
+val dagmap_CONG = store_thm(
+  "dagmap_CONG[defncong]",
+  ``∀f1 f2 g1 g2.
+      (∀d. d ∈ IMAGE action_data (nodeset g1) ⇒ f1 d = f2 d) ∧
+      g1 = g2 ⇒ dagmap f1 g1 = dagmap f2 g2``,
+  simp[PULL_EXISTS] >> ntac 2 gen_tac >>
+  ho_match_mp_tac dag_ind >> simp[polydata_upd_def]);
 
-val dagEVALR_total = store_thm(
-  "dagEVALR_total",
-  ``∀d a. ∃r. dagEVAL opn a d r``,
-  ho_match_mp_tac dag_ind >> rpt strip_tac >> simp[Once dagEVALR_cases] >>
-  metis_tac[]);
+val dagmerge_def = new_specification("dagmerge_def",
+  ["dagmerge"],
+  dag_recursion |> ISPEC ``λa:(α,β)node r g2:(α,β)dag. a <+ r g2``
+                |> SPEC ``λr2:(α,β)dag. r2``
+                |> SIMP_RULE (srw_ss()) [FUN_EQ_THM, dagAdd_commutes'])
+val _ = export_rewrites ["dagmerge_def"]
 
-(*
-val dagEVALR_unique = store_thm(
-  "dagEVALR_unique",
-  ``(∀a b acc. a ≁ₜ b ⇒ opn a (opn b acc) = opn b (opn a acc)) ⇒
-    ∀a d r1.
+val dagmerge_ASSOC = store_thm(
+  "dagmerge_ASSOC",
+  ``∀d1 d2 d3. dagmerge d1 (dagmerge d2 d3) = dagmerge (dagmerge d1 d2) d3``,
+  ho_match_mp_tac dag_ind >> simp[]);
 
-*)
+val dag_recursion' = store_thm(
+  "dag_recursion'",
+  ``∀f e.
+      (∀a b g r. a ≁ₜ b ⇒
+                 f a (b <+ g) (f b g r) = f b (a <+ g) (f a g r)) ⇒
+      ∃h. h emptydag = e ∧
+          ∀a d. h (a <+ d) = f a d (h d)``,
+  rpt gen_tac >>
+  disch_then (strip_assume_tac o
+    MATCH_MP (dag_recursion
+                |> ISPEC ``λa:(α,β)node r:((α,β)dag # γ).
+                             (a <+ FST r, f a (FST r) (SND r) : γ)``
+                |> SPEC ``(emptydag : (α,β)dag, e : γ)``
+                |> SIMP_RULE (srw_ss()) [FORALL_PROD, dagAdd_commutes'])) >>
+  qexists_tac `SND o h` >> simp[] >>
+  `∀d. FST (h d) = d` suffices_by simp[] >>
+  ho_match_mp_tac dag_ind >> simp[]);
+
+val ddel_lemma = prove(
+  ``∀b c g r.
+      b ≁ₜ c ⇒
+      (if a = b then c <+ g else b <+ (if a = c then g else c <+ r)) =
+      (if a = c then b <+ g else c <+ (if a = b then g else b <+ r))``,
+  rw[] >> simp[dagAdd_commutes']);
+
+val ddel_def = new_specification("ddel_def",
+  ["ddel"],
+  MATCH_MP
+    (dag_recursion'
+      |> ISPEC ``λb:(α,β)node g:(α,β)dag r. if a = b then g else b <+ r``
+      |> Q.SPEC `emptydag`
+      |> SIMP_RULE (srw_ss()) [])
+    ddel_lemma
+      |> Q.GEN `a`
+      |> SIMP_RULE bool_ss [SKOLEM_THM]
+      |> SIMP_RULE bool_ss [FORALL_AND_THM]);
+
+val ddel_empty = save_thm("ddel_empty[simp]", CONJUNCT1 ddel_def)
+
+val ddel_simp = save_thm(
+  "ddel_simp[simp]",
+  ddel_def |> CONJUNCT2 |> SPECL [``a:(α,β)node``, ``a:(α,β)node``]
+           |> REWRITE_RULE[]);
+
+val dagAdd_11 = store_thm(
+  "dagAdd_11[simp]",
+  ``(a <+ g = b <+ g ⇔ a = b) ∧ (a <+ g1 = a <+ g2 ⇔ g1 = g2)``,
+  simp[EQ_IMP_THM] >> conj_tac
+  >- (disch_then (mp_tac o Q.AP_TERM `nodebag`) >> simp[]) >>
+  disch_then (mp_tac o Q.AP_TERM `ddel a`) >> simp[]);
+
+val (dagREL_rules, dagREL_ind, dagREL_cases) = Hol_reln`
+  dagREL R ε ε ∧
+
+  ∀a1 a2. R a1 a2 ∧ dagREL R d1 d2 ⇒ dagREL R (a1 <+ d1) (a2 <+ d2)
+`
+
+val dagREL_monotone = store_thm(
+  "dagREL_monotone[mono]",
+  ``(∀a b. R1 a b ⇒ R2 a b) ⇒ dagREL R1 d1 d2 ⇒ dagREL R2 d1 d2``,
+  strip_tac >> map_every qid_spec_tac [`d2`, `d1`] >>
+  Induct_on `dagREL` >> metis_tac[dagREL_rules]);
+
+val dagFOLD_def = new_specification("dagFOLD_def",
+  ["dagFOLD"],
+  dag_recursion |> SIMP_RULE bool_ss [GSYM RIGHT_EXISTS_IMP_THM, SKOLEM_THM]
+                |> CONV_RULE (RENAME_VARS_CONV ["g"] THENC
+                              STRIP_QUANT_CONV (RENAME_VARS_CONV ["f", "acc"])))
+
+val touches_SYM' = prove(``a ∼ₜ b ⇔ b ∼ₜ a``, metis_tac[touches_SYM])
+
+val BAG_FILTER_FILTER = prove(
+  ``BAG_FILTER P (BAG_FILTER Q b) = BAG_FILTER (λa. P a ∧ Q a) b``,
+  simp[BAG_FILTER_DEF] >> simp[FUN_EQ_THM] >> rw[] >> fs[]);
+
+val wave0_def = new_specification("wave0_def",
+  ["wave0"],
+  dag_recursion |> ISPEC ``λa:(α,β)node b:(α,β)node bag.
+                              BAG_INSERT a (BAG_FILTER (λb. a ≁ₜ b) b)``
+                |> SPEC (alpha_node ``EMPTY_BAG``)
+                |> SIMP_RULE (srw_ss()) []
+                |> SIMP_RULE (srw_ss()) [Once touches_SYM', BAG_FILTER_FILTER]
+                |> SIMP_RULE (srw_ss()) [BAG_INSERT_commutes]
+                |> SIMP_RULE (srw_ss()) [Once CONJ_COMM]);
+
 val _ = export_theory();
